Added defn of mgu

mgu.fst
@@ -3,12 +3,19 @@ module Mgu
 open Term
 open Subst
 
+val apply_list_length_lemma : st:subst -> lt:list term -> Lemma
+  (requires true)
+  (ensures ( List.Tot.length lt = List.Tot.length (apply_list st lt)) )
+
+let rec apply_list_length_lemma st lt = match lt with
+  | [] -> ()
+  | hd::tl -> apply_list_length_lemma st tl
+
 val mgu: t1:term -> t2:term -> Tot (option subst)
 val mgu_list : l1:list term -> l2:list term -> Tot (option subst)
 let rec mgu t1 t2 = match t1,t2 with
-  | Var v , Var x -> Some (v,x)
-  | Var v , Name n -> Some(v,n)
-  | Name n, Var v -> Some (v,n)
+  | Var v , x -> Some [(v,x)]
+  | x , Var v -> Some [(v,x)]
   | Func s args1,Func s args2 -> mgu_list args1 args2
   | _,_ -> None
 and mgu_list l1 l2 = match l1,l2 with
@@ -16,5 +23,12 @@ and mgu_list l1 l2 = match l1,l2 with
   | hd1::tl1 , hd2::tl2 -> begin
       let s1 = mgu hd1 hd2 in
       if None? s1 then None
-      else Some ( (Some?.v s1)::( mgu_list (apply_list s1 tl1) (apply_list s1 tl2) ) )
+      else (
+            let s2 = Some?.v s1 in
+            apply_list_length_lemma s2 tl1 ; apply_list_length_lemma s2 tl2;
+            let s3 = mgu_list (apply_list s2 tl1) (apply_list s2 tl2) in
+            if None? s3 then None
+            else Some ( (FStar.List.Tot.hd s2)::( Some?.v s3 ) )
+           )
       end
+  | _,_ -> None
